src/AwsCryptographicMaterialProviders/CMM.dfy
@@ -1,0 +1,32 @@
+
+// Copyright Amazon.com Inc. or its affiliates. All Rights Reserved.
+// SPDX-License-Identifier: Apache-2.0
+
+include "../StandardLibrary/StandardLibrary.dfy"
+include "../Generated/AwsCryptographicMaterialProviders.dfy"
+include "Materials.dfy"
+
+module 
+  {:extern "Dafny.Aws.Crypto.AwsCryptographicMaterialProvidersClient2.CMM"}
+  AwsCryptographicMaterialProviders2.CMM
+{
+  import opened Wrappers
+  import Aws.Crypto
+  import Materials
+
+  trait {:termination false} VerifiableInterface
+    extends Crypto.ICryptographicMaterialsManager
+  {
+    method GetEncryptionMaterials(input: Crypto.GetEncryptionMaterialsInput) 
+      returns (res: Result<Crypto.GetEncryptionMaterialsOutput, string>)
+      ensures res.Success?
+      ==>
+        && Materials.EncryptionMaterialsWithPlaintextDataKey(res.value.encryptionMaterials)
+
+    method DecryptMaterials(input: Crypto.DecryptMaterialsInput) 
+      returns (res: Result<Crypto.DecryptMaterialsOutput, string>)
+      ensures res.Success?
+      ==>
+        && Materials.DecryptionMaterialsWithPlaintextDataKey(res.value.decryptionMaterials)
+  }
+}
